ported MD5 to use the new array interface

examples/low-level/array.fsi
@@ -20,8 +20,12 @@ let testf v = v 1*)
 type array : Type -> Type
 
 (*making it GTot causes a strange error in the postcondition of readIndex *)
-assume val asRef : #a:Type  -> va:(array a) -> Tot (ref (seq a))
+val asRef : #a:Type  -> va:(array a) -> Tot (ref (seq a))
 
+
+val length: #a:Type -> x:array a -> PureMem nat
+  (requires (fun h -> refExistsInMem (asRef x) h))
+  (ensures  (fun h y _ -> refExistsInMem (asRef x) h /\ y=Seq.length (loopkupRef (asRef x) h)))
 
 (*using the 2 definitions below causes a strange error in readIndex amd updIndex*)
 (*val arrayExistsInMem : #a:Type -> (array a) -> smem -> GTot bool
